src/well_formedness.lean
@@ -7,7 +7,7 @@ open rc_correctness.expr
 open rc_correctness.fn_body
 open rc_correctness.lin_type
 
-inductive fn_body_wf (β : const → var → lin_type) (δ : program) : finset var → fn_body → Prop
+inductive fn_body_wf (δ : program) (β : const → var → lin_type) : finset var → fn_body → Prop
 notation Γ ` ⊢ `:1 F := fn_body_wf Γ F
 | ret {Γ : finset var} {x : var} 
   (x_def : x ∈ Γ) :
@@ -17,7 +17,7 @@ notation Γ ` ⊢ `:1 F := fn_body_wf Γ F
   (z_used : z ∈ FV F) (z_undef : z ∉ Γ) (F_wf : insert z Γ ⊢ F) :
   Γ ⊢ (z ≔ c⟦ys…⟧; F)
 | let_const_app_part {Γ : finset var} {z : var} {c : const} {ys : list var} {F : fn_body}
-  (ys_def : ys.to_finset ⊆ Γ) 
+  (ys_def : ys.to_finset ⊆ Γ) (arity_leq : ys.length ≤ (δ c).ys.length)
   (no_𝔹_var : ∀ x : var, β c x ≠ 𝔹) 
   (z_used : z ∈ FV F) (z_undef : z ∉ Γ) (F_wf : insert z Γ ⊢ F) :
   Γ ⊢ (z ≔ c⟦ys…, _⟧; F)
@@ -37,12 +37,12 @@ notation Γ ` ⊢ `:1 F := fn_body_wf Γ F
   (x_def : x ∈ Γ) (Fs_wf : ∀ F ∈ Fs, Γ ⊢ F) :
   Γ ⊢ (case x of Fs)
 
-notation β `; ` δ `; ` Γ ` ⊢ `:1 F := fn_body_wf β δ Γ F
+notation δ `; ` β `; ` Γ ` ⊢ `:1 F := fn_body_wf δ β Γ F
 
-inductive const_wf (β : const → var → lin_type) (δ : program) : const → Prop
+inductive const_wf (δ : program) (β : const → var → lin_type) : const → Prop
 notation `⊢ `:1 c := const_wf c
 | const {c : const}
-  (F_wf : β; δ; (δ c).ys.to_finset ⊢ (δ c).F) (nd_ys : multiset.nodup (δ c).ys) : 
+  (F_wf : δ; β; (δ c).ys.to_finset ⊢ (δ c).F) (nd_ys : multiset.nodup (δ c).ys) : 
   ⊢ c
 
 notation β `; ` δ ` ⊢ `:1 c := const_wf β δ c
@@ -50,7 +50,7 @@ notation β `; ` δ ` ⊢ `:1 c := const_wf β δ c
 inductive program_wf (β : const → var → lin_type) : program → Prop
 notation `⊢ `:1 δ := program_wf δ
 | program {δ : program}
-  (const_wf : ∀ c : const, β; δ ⊢ c) :
+  (const_wf : ∀ c : const, δ; β ⊢ c) :
   ⊢ δ
 
 notation β ` ⊢ `:1 δ := program_wf β δ
